[coq] f

coq/lambda-calculus.v
@@ -1,26 +1,27 @@
-(* ~~~~~~~~~~~~~~~~~~~~~~~~~~~~~~~~~~~~~~~~~~~ *)
-(** * Lambda calculus                          *)
-(* ~~~~~~~~~~~~~~~~~~~~~~~~~~~~~~~~~~~~~~~~~~~ *)
 Require Import Arith.
+Require Import ssreflect.
+Set Nested Proofs Allowed.
 
-(*
-  Some notes from [Pie02]
+(** * λ-calculus term -- 7.1
 
-  To save writing too many parentheses, it exists two conventions when
+Syntax for a λ-calculus with a nameless representation of terms.
+
+Notes from [Pie02]:
+
+- To save writing too many parentheses, it exists two conventions when
   writing lambda-terms in linear form.  First, application associates
   to the left -- that is, `s t u` stands for the same tree as `(s t)
   u`.  Second, the bodies of abstraction are taken to extend as far to
   the right as possible, so that, for example, `λx. λy. x y x` stands
   for the same tree as `λx. (λy. ((x y) x))`.
 
-  This representation avoids renaming by using De Bruijn notation.  It
-  replaces named variables by natural numbers, where the number `k`
-  stands for "the variable bound by the `k`'th enclosing λ". For
-  example, the ordinary term `λx.x` corresponds to the nameless term
-  `λ.0`, while `λx.λy. x (y x)` corresponds to `λ.λ. 1 (0 1)`.
+- The nameless representation avoids renaming by using De Bruijn
+  notation.  It replaces named variables by natural numbers, where the
+  number `k` stands for "the variable bound by the `k`'th enclosing
+  λ". For example, the ordinary term `λx.x` corresponds to the
+  nameless term `λ.0`, while `λx.λy. x (y x)` corresponds to `λ.λ. 1
+  (0 1)`.
 *)
-
-(* Syntax definition -- p.84 *)
 Inductive term: Set :=
 | TmVar: nat -> term
 | TmAbs: term -> term
@@ -30,91 +31,160 @@ Notation "% k" := (TmVar k) (at level 20).
 Infix "@@" := TmApp (at level 25, left associativity).
 Notation "λ∙ t" := (TmAbs t) (at level 35).
 
-(* Some definitions *)
+(** ** Some examples -- 6.1.1 *)
+(* λs. λz. z *)
 Example c0: term := λ∙ λ∙ %0.
+(* λs. λz. s (s z) *)
 Example c2: term := λ∙ λ∙ %1 @@ (%1 @@ %0).
-Example plus: term := λ∙ λ∙ λ∙ λ∙ %3 @@ %1 @@ (%2 @@ %0 @@ %1).
+(* λm. λn. λs. λz. m s (n s z) *)
+Example plus: term := λ∙ λ∙ λ∙ λ∙ %3 @@ %1 @@ (%2 @@ %1 @@ %0).
+(* (plus c2) c0 *)
 Example c2': term := plus @@ c2 @@ c0.
+(* (λx. (λx. x)) (λx. x) *)
+Example foo: term := (λ∙ (λ∙%0)) @@ (λ∙%0).
 
-Require Import Decidable.
+Lemma var_inj: forall k l, TmVar k = TmVar l -> k = l.
+Proof. intros. injection H. trivial. Qed.
 
-(** * n-Terms
+(** * n-Terms -- 6.1.2
 
-- A 0-terms is a term with no free variables
-- A 1-terms is a term with at most one free variable
-- A n-terms is a term with at most n free variables, numbered
-  between 0 and n-1
+The elements of `forall t, (Terms t n)` are terms `t` with at most `n`
+free variables.
 
- *)
+- A 0-Terms is a term with no free variables.
+- A 1-Terms is a term with at most one free variable.
+- A n-Terms is a term with at most n free variables, numbered between
+  0 and n-1.
+*)
+Inductive Terms: term -> nat -> Prop :=
+| TermsVar: forall k n,
+    0 <= k -> k < n ->  Terms (TmVar k) n
+| TermsAbs: forall t n,
+    Terms t (S n) -> Terms (TmAbs t) n
+| TermsApp: forall t1 t2 n,
+    Terms t1 n -> Terms t2 n -> Terms (TmApp t1 t2) n.
 
-(* Fixpoint Terms (t: term) (n: nat): Prop := *)
-(*   match t with *)
-(*   | TmVar k => if lt_dec k n *)
-(*                then True   (* k < n  *) *)
-(*                else False   (* k >= n *) *)
-(*   | TmAbs t => Terms t (n + 1) *)
-(*   | TmApp t1 t2 => *)
-(*     let rh := Terms t1 n in *)
-(*     let lh := Terms t2 n in *)
-(*     if dec_True rh *)
-(*     then True *)
-(*     else False *)
-(*   end. *)
+(** **Unit tests *)
+Example unTerms: Terms (%0) 1 := TermsVar 0 1 (Nat.le_refl 0)  Nat.lt_0_1.
+Example zeroTerms: Terms (λ∙%0) 0 := TermsAbs (%0) 0 unTerms.
+Example zeroTerms': Terms (λ∙λ∙%0 @@ %1) 0.
+Proof.
+  apply TermsAbs. apply TermsAbs. apply TermsApp.
+  - apply TermsVar. Nat.order'. Nat.order'.
+  - apply TermsVar. Nat.order'. Nat.order'.
+Qed.
+Example notZeroTerms: ~ Terms (%0) 0.
+Proof. intro EQ. inversion EQ. apply (Nat.lt_irrefl 0 H1). Qed.
 
-Fixpoint Terms (t: term) (n: nat): Prop :=
-  match t with
-  | TmVar k => if lt_dec k n
-               then True   (* k < n  *)
-               else False   (* k >= n *)
-  | TmAbs t => Terms t (S n)
-  | TmApp t1 t2 =>
-    (Terms t1 n) /\ (Terms t2 n)
-  end.
+(** **Properties *)
 
+(** A term only composed of a var `%k` is obviously a free variable
+(there is no lambda abstraction to bind that variable). Hence, that
+term could not be a member of `0-Terms` the set of term with only
+bound variables. *)
+Lemma never_0_terms_var: forall k, ~ Terms (%k) 0.
+Proof.
+  intros k EQ.
+  inversion EQ.
+  apply (Nat.nlt_0_r k H1).
+Qed.
 
-(* Example nTermsVar: forall (n k: nat), *)
-(*     k < n -> Terms (TmVar k) n. *)
-(* Proof. *)
-(*   simpl. *)
-(*   intros. *)
-(*   set (f := lt_dec k n). *)
-(*   destruct f. *)
-(*   exact I. *)
-(*   exact (n0 H). *)
-(* Qed. *)
+(** A var `%k` member of an n-Terms is obviously a free variable so
+that `n > k`. *)
+Lemma terms_var_lt_k_n: forall k n, Terms (%k) n  -> k < n.
+Proof. intros. inversion H. trivial. Qed.
 
-(* Example nTermsAbs: forall (t: term) (n: nat), *)
-(*     n > 0 -> Terms t n -> Terms (TmAbs t) (pred n). *)
-(* Proof. *)
-(*   simpl. *)
-(*   intros. *)
-(*   rewrite pred_Sn in H0. *)
-(*   admit. *)
-(* Admitted. *)
+(** A var `%k` member of a 1-Terms has only one free-variable such
+that `0 <= k < 1` which implies `k = 0`. *)
+Lemma un_terms_0_var: forall (k: nat), Terms (%k) 1 <-> k = 0.
+  Lemma lt_stric_1: forall n, ~ S n < 1.
+  Proof.
+    intros n EQ.
+    destruct n.
+    - apply (Nat.lt_irrefl 1 EQ).
+    -
+      SearchHead (forall (n m: nat), (S n) < _ -> _).
+      apply lt_S_n in EQ.
+      apply Nat.lt_lt_0 in EQ.
+      SearchHead (forall n, ~ n < n).
+      assert (NEQ_0_0 := Nat.lt_irrefl 0).
+      apply (NEQ_0_0 EQ).
+  Qed.
 
-(* Example nTermsApp: forall (t1 t2: term) (n: nat), *)
-(*     Terms t1 n -> Terms t2 n -> Terms (TmApp t1 t2) n. *)
-(* Proof using Type. *)
-(*   intros t1 t2 n nT1 nT2. simpl. split. apply nT1. apply nT2. *)
-(* Qed. *)
+  Lemma lt_eq_0_1: forall (k: nat), 0 <= k -> k < 1 -> k = 0.
+  Proof.
+    intros k HSupK HLowK.
+    destruct k.
+    - reflexivity.
+    - assert (HFalse := lt_stric_1 k HLowK).
+      contradict HFalse.
+  Qed.
 
+Proof.
+  split.
+  - intros.
+    inversion H.
+    SearchHead (forall n k, 0 <= k -> k < 1 -> 0 = k).
+    exact (lt_eq_0_1 k H1 H2).
+  - intros.
+    rewrite H.
+    exact unTerms.
+Qed.
 
+(** A term `t` that has at most `n` free variables also has at most
+`(s n)` free variables. *)
+Theorem terms_r: forall t n, Terms t n -> Terms t (S n).
 
-(* (* Definition zeroTerms : Terms (λ∙%0) 0 = True. *) *)
-(* (* Definition  zeroTerms':= Terms (λ∙λ∙%0 @@ %1) 0 = True. *) *)
-(* (* Definition  zeroTerms3:= Terms (λ∙λ∙%0 @@ %4) 0 = True. *) *)
-Eval compute in (Terms (λ∙%0) 0).
-Eval compute in (Terms (λ∙λ∙%0 @@ %1) 0).
-Eval compute in (Terms (λ∙λ∙%0 @@ %4) 0).
+  (* Variable case *)
+  Lemma terms_var_r: forall k n, Terms (%k) n -> Terms (%k) (S n).
+  Proof.
+    intros.
+    apply TermsVar.
+    inversion H.
+    - (* 0 <= k *) trivial.
+    - (* k < S n*)
+      assert (LT := terms_var_lt_k_n k n H).
+      SearchHead (forall n m, n < m -> n < S m).
+      apply (Nat.lt_lt_succ_r k n LT).
+  Qed.
 
-(* Lemma zeroTerms: Terms (λ∙%0) 0 = True. *)
-(* Proof using Type. simpl. reflexivity. Qed. *)
+  (* Abstraction case *)
+  Lemma terms_abs_r: forall t n, Terms (λ∙ t) n -> Terms (λ∙ t) (S n).
+  Proof.
+    intros.
+    induction H.
+    -
+      SearchHead (forall n m, n < m -> n < S m).
+      assert (LT := Nat.lt_lt_succ_r k n H0).
+      exact (TermsVar k (S n) H LT).
+    - apply TermsAbs.
+      trivial.
+    - apply TermsApp.
+      trivial. trivial.
+  Qed.
 
-(* (* Lemma zeroTerms': Terms (λ∙λ∙%0 @@ %1) 0 = True. *) *)
-(* (* Proof. simpl. compute. exfalso. contradict. *) *)
+  (* Application case *)
+  Lemma terms_app_r: forall t1 t2 n, Terms (t1 @@ t2) n -> Terms (t1 @@ t2) (S n).
+  Proof.
+    intros.
+    induction H.
+    -
+      SearchHead (forall n m, n < m -> n < S m).
+      assert (LT := Nat.lt_lt_succ_r k n H0).
+      exact (TermsVar k (S n) H LT).
+    - apply TermsAbs.
+      trivial.
+    - apply TermsApp.
+      trivial. trivial.
+  Qed.
 
-(* Lemma notZeroTerms: Terms (λ∙λ∙ %4) 0 = False. *)
-(* Proof. simpl. reflexivity. Qed. *)
+Proof.
+  intros.
+  destruct t.
+  - apply (terms_var_r n0 n H).
+  - apply (terms_abs_r t n H).
+  - apply (terms_app_r t1 t2 n H).
+Qed.
 
 
 (** * Shifting -- 6.2.1
@@ -133,13 +203,13 @@ We could say for `2` that
 λ.(0 1)
      ╰────── 1 is a free variable
 
-And it should remain like this after substitution.
+and it should remain like this after substitution!
 
 When a substitution goes under a λ-abstraction (i.e., `λ.2`), the
 context in which the substitution takes place (i.e., `λ.(0 1)`)
 becomes one variable longer that the original.  Thus we need to
 increment free variables in the substitued term up by one so they
-remain free.  But we should not increment bound variable.  So the
+remain free.  But we should not increment bound variables.  So the
 result of the previous substitution is:
 
 [2 ↦ λ.(0 1)] λ.2
@@ -147,43 +217,71 @@ result of the previous substitution is:
     ╰─┴╴│──── The first variable *remains* a bound variable to `λ`
         ╰──── The second variable *remains* free
 
-We use the following notation `↑c,d(k)` for increment variables of `k`
+We use the following notation `↑c,d[t]` for increment variables of `t`
 by `d` level with `c` is the index of the first free variable.  All
 identifiers `k < c` in `t` are bound a so should not be shifted, while
 identifiers `k >= c` in `t` are free and should be shifted.
 
 Shift term by `d`
-↑c,d(k)     = k              if k < c    [1]
-↑c,d(k)     = k + d          if k >= c   [2]
-↑c,d(λ.t)   = λ.↑c+1,d(t)               [3]
-↑c,d(t1 t2) = ↑c,d(t1) ↑c,d(t2)        [4]
+↑c,d[k]     = k              if k < c    (1)
+↑c,d[k]     = k + d          if k >= c   (2)
+↑c,d[λ.t]   = λ.↑c+1,d[t]               (3)
+↑c,d[t1 t2] = ↑c,d[t1] ↑c,d[t2]        (4)
 
 For instance:
 
-↑0,1 `λ.(0 1)` =3⇒ `λ.`↑1,1 `(0 1)`
-                =4⇒ `λ.(`↑1,1`0` ↑1,1`1` `)`
-                =1⇒ `λ.(0` ↑1,1`1` `)`
-                =2⇒ `λ.(0 2)`
-
-We also write ↑1(t) for ↑0,1(t) *)
+↑0,1[λ.(0 1)] =3⇒ λ.↑1,1[(0 1)]
+               =4⇒ λ.(↑1,1[0] ↑1,1[1])
+               =1⇒ λ.(0 ↑1,1[1])
+               =2⇒ λ.(0 2)
+*)
 Fixpoint shift_walk (c: nat) (d: nat) (t: term): term :=
   match t with
-  | TmVar k => if lt_dec k c
-               then TmVar k        (* k < c  *)
-               else TmVar (k + d)  (* k >= c *)
+  | TmVar k => match lt_dec k c with
+              | left _ => TmVar k        (* k < c  *)
+              | _      => TmVar (k + d)  (* k >= c *)
+              end
   | TmAbs t => TmAbs (shift_walk (S c) d t)
   | TmApp t1 t2 =>
     let t1' := shift_walk c d t1 in
     let t2' := shift_walk c d t2 in
     TmApp t1' t2'
   end.
-Definition shift (d: nat) (t: term)   := shift_walk 0 d t.
+
+
+(* We also write ↑1[t] for ↑0,1[t] *)
+Definition shift (d: nat) (t: term) := shift_walk 0 d t.
+
+Compute (match lt_dec 0 1 with
+         | left _  => true
+         | right _ => false
+        end).
 
 Eval compute in (shift 1 (λ∙ %0 @@ %1)).
 Eval compute in (shift 2 (λ∙ λ∙ %1 @@ %0 @@ %2)).
 Eval compute in (shift 2 (λ∙ %0 @@ %1 @@ (λ∙ %0 @@ %1 @@ %2))).
 
-Eval compute in (eq_nat 2 (1 + 3)).
+
+(* Errata  *)
+(* p 79, exercise 6.2.3 *)
+
+(*     The statement to be shown is not quite true for d < 0.  To be true for *)
+(*     n>=0 and any integral d, it should be "Show that, if t is an n-term and, *)
+(*     if d < 0, the free variables of t are all at least |d|, then <shift t up *)
+(*     by d above cutoff c> is a (max(n+d,0))-term." *)
+
+Lemma shift_zero: forall t c, shift_walk c 0 t = t.
+Proof.
+  intros.
+  elim: t c.
+  - intros. simpl. destruct (lt_dec n c).
+    + reflexivity.
+    + assert (EQ:=Nat.add_0_r n). rewrite EQ. reflexivity.
+  - simpl. congruence.
+  - simpl. congruence.
+Qed.
+
+
 (** * Substitution -- 6.2.4
 
 The substitution of a term `s` for a variable number `j` in a term
@@ -192,9 +290,10 @@ The substitution of a term `s` for a variable number `j` in a term
 *)
 (* Fixpoint substitute_walk (c: nat) (j: nat) (s t: term) : term := *)
 (*   match t with *)
-(*   | TmVar k => if eq_nat_dec k (j + c) *)
-(*                then (shift c s)  (* k = j+c *) *)
-(*                else TmVar k      (* k != j  *) *)
+(*   | TmVar k => match eq_nat_dec k (j + c) with *)
+(*                | right _ => (shift c s)  (* k = j+c *) *)
+(*                | left  _ => TmVar k      (* k != j  *) *)
+(*               end *)
 (*   | TmAbs t => TmAbs (substitute_walk (S c) j s t) *)
 (*   | TmApp t1 t2 => *)
 (*     let t1' := substitute_walk c j s t1 in *)
@@ -204,15 +303,21 @@ The substitution of a term `s` for a variable number `j` in a term
 (* Definition substitute (j: nat) (s t: term) := substitute_walk 0 j s t. *)
 Fixpoint substitute (j: nat) (s t: term) : term :=
   match t with
-  | TmVar k => if eq_nat_dec k j
-               then s            (* k = j+c *)
-               else TmVar k      (* k != j  *)
+  | TmVar k => match eq_nat_dec k j with
+               | left  _ => s            (* k =  j *)
+               | _       => TmVar k      (* k != j  *)
+              end
   | TmAbs t => TmAbs (substitute (S j) (shift 1 s) t)
   | TmApp t1 t2 =>
     let t1' := substitute j s t1 in
     let t2' := substitute j s t2 in
     TmApp t1' t2'
   end.
+
+Compute (match eq_nat_dec 0 0 with
+         | left _  => true
+         | right _ => false
+        end).
 
 (*
   Γ = z ↦ 5, y ↦ 4, x ↦ 3, w ↦ 2, b ↦ 1, a ↦ 0.
@@ -228,35 +333,102 @@ Eval compute in (substitute 1 (%0) (λ∙%2 @@ %0)).
 (* [x ↦ (λz. z w)](λy.x) = λy.λz. z w *)
 Eval compute in (substitute 3 (λ∙ %6 @@ %3) (λ∙%4)).
 
-Fixpoint isval (t: term): bool :=
+Fixpoint unshift_walk (c: nat) (t: term): term :=
   match t with
-  | TmAbs _ => true
-  | _ => false
-  end.
-
-
-
-Fixpoint eval (t: term): option term :=
-  match t with
-  | TmApp (TmAbs t11) v2 =>
-    if isval v2 then Some (termSubstTop v2 t11)
-    else None
+  | TmVar k => match lt_dec k c with
+               | left _ => TmVar k         (* k < c  *)
+               | _      => TmVar (pred k)  (* k >= c *)
+              end
+  | TmAbs t => TmAbs (unshift_walk (S c) t)
   | TmApp t1 t2 =>
-    match isval t1 with
-    | true =>
-      match eval t2 with
-      | Some t2' => Some (TmApp t1 t2')
-      | _ => None
-      end
-    | false =>
-      match eval t1 with
-      | Some t1' => Some (TmApp t1' t2)
-      | _ => None
-      end
-    end
-  | _ => None
+    let t1' := unshift_walk c t1 in
+    let t2' := unshift_walk c t2 in
+    TmApp t1' t2'
+  end.
+Definition unshift t: term := unshift_walk 0 t.
+
+Fixpoint eval1 (t: term) {struct t}: option term :=
+  let isval := fun (t: term) =>
+                 match t with
+                 | TmAbs _ => true
+                 | _       => false
+                 end
+  in match t with
+     (* E-AppAbs*)
+     | TmApp (TmAbs t12) v2 =>
+       if isval v2
+       then let t' := substitute 0 (shift 1 v2) t12
+            in Some (unshift t')
+       else None
+     | TmApp t1 t2 =>
+       if isval t1
+       (* E-App2 *)
+       then match eval1 t2 with
+            | Some t2' => Some (TmApp t1 t2')
+            | _        => None
+            end
+       (* E-App1 *)
+       else match eval1 t1 with
+            | Some t1' => Some (TmApp t1' t2)
+            | _        => None
+            end
+     | _ => None
+     end.
+
+Fixpoint eval (t: term): term :=
+  match t with
+    | TmVar k => t
+    | TmApp (TmAbs t1) t2 =>
+      let v := (eval t2)
+      in unshift (substitute 0 (shift 1 v) t1)
+    | TmApp t1 t2 => TmApp (eval t1) (eval t2)
+    | TmAbs t => TmAbs (eval t)
   end.
 
+Inductive isVal : term -> Set :=
+  | here t1 : isVal (TmAbs t1).
+
+Hint Constructors isVal.
+
+Inductive betared1 : term -> term -> Set :=
+  | betared1appabs t1 t2 : isVal t2 -> betared1 ((λ∙ t1) @@ t2)  (unshift (substitute 0 (shift 1 t2) t1))
+  | betared1app2 t1 t2 t2' : isVal t1 -> betared1 t2 t2' -> betared1 (t1 @@ t2) (t1 @@ t2')
+  | betared1app1 t1 t2 t1' : betared1 t1 t1' -> betared1 (t1 @@ t2) (t1' @@ t2).
+
+Hint Constructors betared1.
+
+Compute (eval ((λ∙ %1 @@ %0 @@ %2) @@ (λ∙%0))).
+
+Example test : betared1 ((λ∙ %1 @@ %0 @@ %2) @@ (λ∙%0)) (%0 @@ (λ∙%0) @@ %1).
+Proof.
+  auto with betared1.
 
 
-  end.
+
+Compute (eval c2).
+(* c0 = λs. λz. z *)
+(* plus = λm. λn. λs. λz. m s (n s z) *)
+(* plus @@ c0 @@ c0 = (λm. λn. λs. λz. m s (n s z)) (λs. λz. z) (λs. λz. z)
+                    ~ (λ . λ . λ . λ . 3 1 (2 1 0)) (λ . λ . 0) (λ . λ . 0)
+            AppAbs => (λn. λs. λz. (λs. λa. a) s (n s z)) (λs. λz. z)
+                    ~ (λ . λ . λ . (λ . λ . 0) 1 (2 1 0)) (λ . λ . 0)
+            AppAbs => λs. λz. (λs. λa. a) s ((λs. λa. a) s z)
+                    ~ λ . λ . (λ . λ . 0) 1 ((λ . λ . 0) 1 0)
+
+*)
+(* plus @@ c0 @@ c0 = (λm. λn. λs. λz. m s (n s z)) (λs. λz. z) (λs. λz. z)
+                    ~ (λ . λ . λ . λ . 3 1 (2 1 0)) (λ . λ . 0) (λ . λ . 0)
+            AppAbs => (λn. λs. λz. (λs. λa. a) s (n s z)) (λs. λz. z)
+                    ~ (λ . λ . λ . (λ . λ . 0) 1 (2 1 0)) (λ . λ . 0)
+            AppAbs => λs. λz. (λs. λa. a) s ((λs. λa. a) s z)
+                    ~ λ . λ . (λ . λ . 0) 1 ((λ . λ . 0) 1 0)
+*)
+
+Example c0': term := (plus @@ c0 @@ c0).
+Compute (eval1 c0').
+Compute (eval c0').
+Compute (eval (eval (eval (eval c0')))).
+Compute (eval c2').
+
+Extraction Language Scheme.
+Extraction eval1.
